SystemF2Effect: work on region handle freshness
Ignore-this: d56dc5f86e0f70fe35baec8e9ec236d8

darcs-hash:20130122063136-08f32-d098d35d0af0f574f9c63cfed12239bb8e1e1688

devel/Iron/Language/SystemF2Effect/Store/Prop.v
@@ -1,5 +1,5 @@
 
-
+Require Import Iron.Language.SystemF2Effect.Base.
 
 Inductive stprop :=
  (* A region descriptor.
@@ -9,3 +9,219 @@ Inductive stprop :=
 
 Definition stprops 
  := list stprop.
+
+
+
+Fixpoint max_list (xs : list nat) :=
+ match xs with
+ |  nil     => 0
+ |  x :: xs => max x (max_list xs)
+ end.
+
+
+Lemma max_ge_left1
+ : forall a b
+ , max a b >= a.
+Proof.
+ intros. gen b.
+ induction a; intros.
+  omega.
+  simpl. break b.
+   omega.
+   cut (max a X >= a). 
+    snorm. omega.
+   eauto.
+Qed.
+
+
+Lemma max_ge_above
+ : forall a b c
+ ,  a >= b
+ -> max c a >= b.
+Proof.
+ intros. gen a b.
+ induction c; intros. 
+  snorm.
+  snorm. break a.
+   omega.
+   subst.
+   destruct b.   
+    omega.   
+    have (X >= b) by omega.
+    spec IHc H0. omega.
+Qed. 
+
+
+Lemma max_ge_left
+ : forall a b c
+ , c >= max a b -> c >= a.
+Proof.
+ intros. gen b c.
+ induction a; intros.
+  snorm.
+   snorm. break b.
+   subst. auto.
+   destruct c.
+    nope.
+    have (c >= max a X) by omega.
+    lets D: IHa H0. omega.
+Qed.
+Hint Resolve max_ge_left.
+
+
+Lemma max_ge_right
+ : forall a b c
+ , c >= max a b -> c >= b.
+Proof.
+ intros. gen b c.
+ induction a; intros.
+  snorm. subst. auto.
+  simpl in H.
+  destruct b.
+   simpl in H. subst. auto.
+   destruct c.
+    nope.
+    have (c >= max a b) by omega.
+    lets D: IHa H0. omega.
+Qed.
+Hint Resolve max_ge_right.
+
+
+Lemma max_list_above
+ :  forall xs
+ ,  Forall (fun x => max_list xs >= x) xs.
+Proof.
+ intros.
+ induction xs; unfold not; intros.
+  snorm.
+  eapply Forall_cons.
+   snorm. eauto.
+   eapply Forall_impl
+    with (P := (fun x => max_list xs >= x)); eauto.
+   intros.
+   simpl.
+   remember (max_list xs) as mx.
+   eapply max_ge_above. auto.
+Qed.
+
+
+Lemma max_list_succ_not_in
+ :  forall xs
+ ,  not (In (S (max_list xs)) xs).
+Proof.
+ intros.
+ unfold not. intros.
+ lets D1: max_list_above xs.
+ norm.
+ spec D1 H. omega.
+Qed.
+
+
+Lemma list_in_map
+ :  forall {A B} (x : A) (xs : list A) (f : A -> B)
+ ,  In x xs -> In (f x) (map f xs).
+Proof.
+ intros. gen x f.
+ induction xs; intros.
+  simpl. auto.
+  simpl. simpl in H.
+   inverts H.
+    left.  auto.
+    right. auto.
+Qed.
+
+
+Fixpoint regionOfStProp (s : stprop) : option nat :=
+ match s with
+ | SRegion n       => Some n
+ end.
+
+
+Fixpoint catOptions {A} (xs : list (option A)) : list A
+ := match xs with
+    | nil             => nil
+    | Some x :: rest  => x :: catOptions rest
+    | None   :: rest  => catOptions rest
+    end.
+
+
+Definition allocRegion (sp : stprops) : nat 
+ := S (max_list (catOptions (map regionOfStProp sp))).
+
+
+Lemma max_weaken_left
+ :  forall a b c
+ ,        a >= b
+ -> max c a >= b.
+Proof.
+ intros. gen a b.
+ induction c; intros.
+  snorm.
+  simpl. destruct a.
+   omega.
+   destruct b.
+    omega.
+    cut (max c a >= b). intros. omega.
+     eapply IHc. omega.
+Qed.
+
+
+Lemma allocRegion_weaken
+ :  forall sp s n
+ ,  allocRegion sp        >= n
+ -> allocRegion (sp :> s) >= n.
+Proof.
+ intros.
+  destruct n.
+  omega.
+  unfold allocRegion in *.
+   snorm.
+   have (max_list (catOptions (map regionOfStProp sp)) >= n) by omega. clear H.
+   cut  (max n0 (max_list (catOptions (map regionOfStProp sp))) >= n).
+    intros. omega.
+    apply max_weaken_left. 
+    auto.
+Qed.
+ 
+
+Lemma allocRegion_above
+ : forall sp
+ , Forall (fun s => match regionOfStProp s with
+                    | Some n => allocRegion sp > n
+                    | None   => True
+                    end)
+          sp.
+Proof.
+ induction sp; intros.
+  snorm.
+  snorm.
+  inverts H.
+   destruct x.
+    snorm.
+    unfold allocRegion.
+     simpl.
+     remember (max_list (catOptions (map regionOfStProp sp))) as X.
+     cut (max n0 X >= n0). 
+      intros. omega.
+     apply max_ge_left1.
+   destruct x.
+    snorm. 
+    spec IHsp H0.
+    snorm.
+    apply allocRegion_weaken. auto.
+Qed.
+
+
+(* Allocated region is fresh wrt existing store properties. *)
+Lemma allocRegion_fresh
+ : forall sp
+ , not (In (SRegion (allocRegion sp)) sp).
+Proof.
+ intros.
+ unfold not. intros.
+ lets D: allocRegion_above sp.
+  snorm.
+ spec D H.
+  snorm. omega.
+Qed.
+ 
